Phew! H1-H2 predicates are indeed designs :)

theories/theories/utp_designs.thy
@@ -93,7 +93,7 @@ definition Mk_ALPHA_FUNCTION ::
 definition "H1   \<equiv> \<lambda> p. `ok \<Rightarrow> p`"
 definition "J a  \<equiv> `(ok \<Rightarrow> ok') \<and> II\<^bsub>a -\<^sub>f OK\<^esub>`"
 definition "H2  \<equiv> \<lambda> p. [p\<^sup>t \<Rightarrow>\<alpha> (p\<^sup>f)]\<alpha>"
-definition "H2' \<equiv> \<lambda> p. (p ;\<alpha> J (\<alpha> p))"
+definition "H2' \<equiv> \<lambda> p. (p ;\<alpha> J (homr (\<alpha> p)))"
 definition "H3  \<equiv> \<lambda> p. `p ; IID\<^bsub>\<alpha> p\<^esub>`"
 definition "H4  \<equiv> \<lambda> p. `p ; true\<^bsub>\<alpha> p\<^esub> \<Rightarrow> true\<^bsub>\<alpha> p\<^esub>`"
 
@@ -149,6 +149,42 @@ lemma DESIGN_ALPHABET_finsert [simp]:
   "a \<in> DESIGN_ALPHABET \<Longrightarrow> finsert okay a = a"
   "a \<in> DESIGN_ALPHABET \<Longrightarrow> finsert okay' a = a"
   by (auto simp add:DESIGN_ALPHABET_def)
+
+lemma DESIGN_ALPHABET_REL_ALPHABET [closure]:
+  "a \<in> DESIGN_ALPHABET \<Longrightarrow> a \<in> REL_ALPHABET"
+  apply (unfold DESIGN_ALPHABET_def)
+  apply (auto)
+done
+
+lemma DESIGN_ALPHABET_ok [closure]:
+  "a \<in> DESIGN_ALPHABET \<Longrightarrow> okay \<in>\<^sub>f a"
+  apply (unfold DESIGN_ALPHABET_def)
+  apply (auto)
+done
+
+lemma DESIGN_ALPHABET_ok' [closure]:
+  "a \<in> DESIGN_ALPHABET \<Longrightarrow> okay' \<in>\<^sub>f a"
+  apply (unfold DESIGN_ALPHABET_def)
+  apply (auto)
+done
+
+lemma DESIGN_ALPHABET_homr [closure]:
+  "a \<in> DESIGN_ALPHABET \<Longrightarrow> homr a \<in> DESIGN_ALPHABET"
+  apply (unfold DESIGN_ALPHABET_def)
+  apply (simp add:closure)
+  apply (auto simp add:hom_right_def closure)
+  apply (metis Int_iff imageI okay_simps(8) out_vars_def undash_dash)
+  apply (metis IntI okay_simps(8) out_vars_def)
+done
+
+lemma DESIGN_ALPHABET_homl [closure]:
+  "a \<in> DESIGN_ALPHABET \<Longrightarrow> homl a \<in> DESIGN_ALPHABET"
+  apply (unfold DESIGN_ALPHABET_def)
+  apply (simp add:closure)
+  apply (auto simp add:hom_left_def closure)
+  apply (metis Int_iff in_vars_def okay_simps(7))
+  apply (metis Int_iff imageI in_vars_def okay_simps(7))
+done
 
 lemma extreme_point_true:
   "`false\<^bsub>a \<^esub>\<turnstile> false\<^bsub>a\<^esub>` = `false\<^bsub>a\<^esub> \<turnstile> true\<^bsub>a\<^esub>`"
@@ -278,9 +314,22 @@ lemma H1_idempotent: "H1 (H1 p) = H1 p"
   apply (utp_pred_tac)
 done
 
+lemma H1_DesignD: "p \<turnstile> q is H1 healthy"
+  apply (simp add:DesignD_def H1_def is_healthy_def)
+  apply (utp_alpha_tac2)
+  apply (utp_pred_auto_tac)
+done
+
 lemma ClosureA_intro: "\<lbrakk> \<alpha> p = \<alpha> q; [p \<Leftrightarrow> q] \<rbrakk> \<Longrightarrow> p = q"
   apply (utp_alpha_tac)
   apply (utp_pred_tac)
+done
+
+lemma eq_iff_taut: "\<lbrakk> \<alpha> P = \<alpha> Q \<rbrakk> \<Longrightarrow> P = Q \<longleftrightarrow> taut (P \<Leftrightarrow>\<alpha> Q)"
+  apply (auto)
+  apply (utp_alpha_tac)
+  apply (rule ClosureA_intro)
+  apply (auto)
 done
 
 lemma AndA_OrA_dist:
@@ -446,334 +495,170 @@ proof -
     by simp
 qed
 
-lemma 
+lemma okay_true_alphabet [alphabet]: "\<alpha> (P\<^sup>t) = \<alpha> P -\<^sub>f \<lbrace>okay'\<rbrace>"
+  by (auto simp add:alphabet)
+
+lemma okay_false_alphabet [alphabet]: "\<alpha> (P\<^sup>f) = \<alpha> P -\<^sub>f \<lbrace>okay'\<rbrace>"
+  by (auto simp add:alphabet)
+
+lemma H2_equivalence:
   assumes "P \<in> WF_RELATION" "\<alpha> P \<in> DESIGN_ALPHABET"
-          "\<alpha> P \<in> HOM_ALPHABET" 
-  shows "P = P ;\<alpha> J (\<alpha> P) \<longleftrightarrow> taut (P\<^sup>f \<Rightarrow>\<alpha> (P\<^sup>t))"
+          "a \<in> HOM_ALPHABET" "in\<^sub>\<alpha> a = undash `\<^sub>f out\<^sub>\<alpha> (\<alpha> P)"
+  shows "[P \<Leftrightarrow>\<alpha> (P ;\<alpha> J a)]\<alpha> = [P\<^sup>f \<Rightarrow>\<alpha> (P\<^sup>t)]\<alpha>"
 proof -
-  have igd: "in\<^sub>\<alpha> (\<alpha> P) = undash `\<^sub>f out\<^sub>\<alpha> (\<alpha> P)"
-    sorry
 
-  with assms have "P = P ;\<alpha> J (\<alpha> P) = (P = P\<^sup>f \<or>\<alpha> (P\<^sup>t \<and>\<alpha> ok'))"
-   apply (unfold J_split[OF assms(1) assms(2) assms(3) igd])
-   apply (simp)
-  done
-
-  also have "... \<longleftrightarrow> taut (P\<^sup>f \<Rightarrow>\<alpha> (P\<^sup>t))"
-    apply (utp_alpha_tac)
-    apply (utp_pred_tac)
-    apply (utp_expr_tac)
-    apply (auto)
-
-  apply (simp add:H2_def H2'_def)
-  apply (subgoal_tac )
-   apply (unfold J_split[OF assms(1) assms(2) assms(3)])
-  apply (utp_alpha_tac)
-  apply (auto)
-
-
-lemma H2_idempotent: "p \<in> WF_RELATION \<Longrightarrow> H2 (H2 p) = H2 p"
-  apply (simp add:H2_def)
-  apply (utp_alpha_tac2)
-  apply (utp_pred_tac)
-  apply (utp_expr_tac)
-  apply (auto)
-done
-
-
-
-lemma H1_DesignD: "p \<turnstile> q is H1 healthy"
-  apply (simp add:DesignD_def H1_def)
-  apply (utp_alpha_tac2)
-  apply (utp_pred_auto_tac)
-done
-
-
-
-lemma H2_H2': "P is H2 healthy \<longleftrightarrow> taut ([P\<^sup>t \<Rightarrow>\<alpha> (P\<^sup>f)]\<alpha>)"
-proof -
-  have "P is H2 healthy \<longleftrightarrow> P = P ;\<alpha> J (\<alpha> P)"
-    by (simp add: H2_def)
-  
-  also have "... = 
-
-  apply (simp add:H2_def H2'_def J_def)
-  apply (utp_pred_auto_tac)
-  apply (utp_rel_auto_tac)
-
-lemma H2_idempotent: "H2 (H2 p) = H2 p"
-  apply (simp add:H2_def J_def)
-  apply (utp_rel_auto_tac)
-done
-
-lemma J_H2: "H2 J = J"
-  apply (simp add:H2_def J_def)
-  apply (utp_rel_auto_tac)
-done
-
-lemma H2_DesignD: "p \<turnstile> q is H2 healthy"
-  apply (simp add:DesignD_def H2_def J_def)
-  apply (utp_rel_auto_tac)
-  apply (auto simp add: EvalR_UNIV)
-
-lemma H1_H2_commute: "H1 (H2 p) = H2 (H1 p)"
-  apply (simp add:H1_def H2_def J_def)
-  apply (utp_rel_auto_tac)
-oops
-
-lemma H3_idempotent: "H3 (H3 p) = H3 p"
-  apply (simp add:H3_def SkipD_def DesignD_def)
-  apply (utp_rel_tac)
-  apply (auto)
-oops
-
-lemma H4_idempotent: "H4 (H4 p) = H4 p"
-  apply (simp add:H4_def)
-  apply (utp_rel_tac)
-  apply (auto)
-
-done
-
-
-(*
-definition DESIGN_ALPHABET :: "'TYPE ALPHABET set"
-where "DESIGN_ALPHABET = REL_ALPHABET \<inter> {a. OK \<subseteq> a}"
-
-
-{a. a \<in> WF_ALPHABET \<and> a \<subseteq> UNDASHED \<union> DASHED \<and> OK \<subseteq> a}"
-*)
-
-(*
-definition DESIGNS :: "('VALUE, 'TYPE) UTP_THEORY" where
-"DESIGNS = \<lparr> utp_alphabets = WF_DESIGN_ALPHABET
-           , healthconds = {H1, H2, H3, H4} \<rparr>"
-
-definition WF_DESIGN where "WF_DESIGN = TheoryPreds DESIGNS"
-*)
-
-subsection {* Basic Laws *}
-
-theorem WF_DESIGN_ALPHABET [closure]:
-"a \<in> DESIGN_ALPHABET \<Longrightarrow> a \<in> REL_ALPHABET"
-  by (simp add:DESIGN_ALPHABET_def)
-
-theorem WF_DESIGN_UNDASHED_DASHED [closure]:
-"a \<in> DESIGN_ALPHABET \<Longrightarrow> a \<subseteq> UNDASHED \<union> DASHED"
-  by (simp add:DESIGN_ALPHABET_def REL_ALPHABET_def)
-
-theorem okay_DESIGN_ALPHABET [elim]: 
-"\<lbrakk> a \<in> DESIGN_ALPHABET; okay \<in> a \<Longrightarrow> P \<rbrakk> \<Longrightarrow> P"
-  by (simp add:DESIGN_ALPHABET_def)
-
-theorem okay'_DESIGN_ALPHABET [elim]: 
-"\<lbrakk> a \<in> DESIGN_ALPHABET; okay' \<in> a \<Longrightarrow> P \<rbrakk> \<Longrightarrow> P"
-  by (simp add:DESIGN_ALPHABET_def)
-
-theorem UNDASHED_okay [simp]: "okay \<in> UNDASHED" 
-  by (simp add:okay_def UNDASHED_def)
-
-theorem DASHED_okay' [simp]: "okay' \<in> DASHED" 
-  by (simp add:okay'_def DASHED_def)
-
-subsection {* Basic Alphabet Laws *}
-
-theorem ok_alphabet [alphabet]:
-"a \<in> DESIGN_ALPHABET \<Longrightarrow> \<alpha> (ok a) = a"
-  by (auto simp add:alphabet closure)
-
-theorem ok'_alphabet [alphabet]:
-"a \<in> DESIGN_ALPHABET \<Longrightarrow> \<alpha> (ok' a) = a"
-  by (auto simp add:alphabet closure)
-
-theorem DesignD_alphabet [alphabet]: 
-"\<lbrakk>r1 \<in> WF_ALPHA_PREDICATE;
-  r2 \<in> WF_ALPHA_PREDICATE;
-  \<alpha> r1 = \<alpha> r2\<rbrakk> \<Longrightarrow>
-  \<alpha> (r1 \<turnstile> r2) = \<alpha> r1 \<union> \<alpha> r2 \<union> OK"
-  apply (simp add:DesignD_def)
-  apply (simp add:alphabet closure)
-  apply (force)
-done
-
-theorem SkipD_alphabet [alphabet]: "a \<in> REL_ALPHABET \<Longrightarrow> \<alpha> (IID a) = a \<union> OK"
-  by (simp add: SkipD_def alphabet closure)
-
-subsection {* Basic Closure Laws *}
-
-lemma ok_pred [closure]: 
-"\<lbrakk> a \<in> WF_ALPHABET; a \<subseteq> UNDASHED \<union> DASHED \<rbrakk> \<Longrightarrow> ok a \<in> WF_RELATION"
-  by (force intro:WF_RELATION_intro simp add:closure alphabet)
-
-lemma ok'_pred [closure]: 
-"a \<in> WF_ALPHABET \<Longrightarrow> ok' a \<in> WF_ALPHA_PREDICATE"
-  by (simp add:closure)
-
-lemma DesignD_rel_closure [closure]: 
-"\<lbrakk> r1 \<in> WF_RELATION; r2 \<in> WF_RELATION; \<alpha> r1 = \<alpha> r2 \<rbrakk> \<Longrightarrow>
-r1 \<turnstile> r2 \<in> WF_RELATION"
-  apply (auto intro:closure simp add:DesignD_def WF_RELATION_def)
-  apply (simp add:REL_ALPHABET_def)
-  apply (simp add:alphabet closure)
-done
-
-lemma SkipD_closure [closure]: "a \<in> REL_ALPHABET \<Longrightarrow> IID a \<in> WF_RELATION"
-  by (simp add:SkipD_def closure alphabet)
-
-lemma J_closure [closure]: "a \<in> DESIGN_ALPHABET \<Longrightarrow> J a \<in> WF_RELATION"
-  by (rule WF_RELATION_intro, simp_all add:closure alphabet J_def)
-
-subsection {* Laws from the notes *}
-
-theorem DesignD_extreme_point_true:
-  assumes "a \<in> DESIGN_ALPHABET"
-  shows "false a \<turnstile> false a = false a \<turnstile> true a"
-  apply (insert assms)
-  apply (simp add:DesignD_def closure alphabet)
-  apply (utp_alpha_tac, utp_pred_auto_tac)
-done
-
-theorem DesignD_extreme_point_nok:
-  assumes "a \<in> DESIGN_ALPHABET"
-  shows "true a \<turnstile> false a = \<not>\<alpha> ok a"
-proof -
-  from assms have "true a \<turnstile> false a = (ok a \<and>\<alpha> true a \<Rightarrow>\<alpha> ok' a \<and>\<alpha> false a)"
-    by (simp add:DesignD_def closure alphabet)
-
-  also from assms have "... = ok a \<Rightarrow>\<alpha> ok' a \<and>\<alpha> false a"
-    by (utp_alpha_tac, utp_pred_auto_tac)
-  
-  also from assms have "... = ok a \<Rightarrow>\<alpha> false a"
-    by (utp_alpha_tac, utp_pred_auto_tac)
-
-  ultimately show ?thesis using assms
-    apply (utp_alpha_tac, utp_pred_auto_tac)
-  done
-qed
-
-theorem DesignD_export_precondition:
-  assumes "p \<in> WF_RELATION" "q \<in> WF_RELATION" "\<alpha> p = \<alpha> q"
-  shows "p \<turnstile> q = p \<turnstile> p \<and>\<alpha> q"
-proof -
-  from assms have "p \<turnstile> q = ok (\<alpha> p) \<and>\<alpha> p \<Rightarrow>\<alpha> ok' (\<alpha> q) \<and>\<alpha> q"
-    by (simp add:DesignD_def closure alphabet)
-
-  also from assms have "... = ok (\<alpha> p) \<and>\<alpha> p \<Rightarrow>\<alpha> ok' (\<alpha> q) \<and>\<alpha> p \<and>\<alpha> q"
-    by (utp_alpha_tac, utp_pred_auto_tac)
-
-  ultimately show ?thesis using assms
-    by (simp add:DesignD_def closure alphabet)
-qed
-
-theorem DesignD_refinement:
-  assumes "p1 \<in> WF_RELATION" "p2 \<in> WF_RELATION" 
-          "q1 \<in> WF_RELATION" "q2 \<in> WF_RELATION"
-          "\<alpha> p1 = \<alpha> q1" "\<alpha> q1 = \<alpha> p2" "\<alpha> p2 = \<alpha> q2" 
-  shows   "(p1 \<turnstile> q1) \<sqsubseteq>\<alpha> (p2 \<turnstile> q2) = [p1 \<Rightarrow>\<alpha> p2]\<alpha> \<and>\<alpha> [p1 \<and>\<alpha> q2 \<Rightarrow>\<alpha> q1]\<alpha>"
-proof -
-  from assms have "(p1 \<turnstile> q1) \<sqsubseteq>\<alpha> (p2 \<turnstile> q2) = [(p2 \<turnstile> q2) \<Rightarrow>\<alpha> (p1 \<turnstile> q1)]\<alpha>"
-    by (simp add:RefA_lemma closure alphabet)
+  from assms have "[P \<Leftrightarrow>\<alpha> (P ;\<alpha> J a)]\<alpha> = [P \<Leftrightarrow>\<alpha> (P\<^sup>f \<or>\<alpha> (P\<^sup>t \<and>\<alpha> ok'))]\<alpha>"
+    by (simp add:J_split)
 
   also from assms 
-  have "... = [(ok (\<alpha> p2) \<and>\<alpha> p2 \<Rightarrow>\<alpha> ok' (\<alpha> q2) \<and>\<alpha> q2) \<Rightarrow>\<alpha> (ok (\<alpha> p1) \<and>\<alpha> p1 \<Rightarrow>\<alpha> ok' (\<alpha> q1) \<and>\<alpha> q1)]\<alpha>"
-    by (simp add:DesignD_def closure alphabet)
-  
+  have "... = [((P \<Leftrightarrow>\<alpha> (P\<^sup>f \<or>\<alpha> (P\<^sup>t \<and>\<alpha> ok')))\<^sup>f) \<and>\<alpha> ((P \<Leftrightarrow>\<alpha> (P\<^sup>f \<or>\<alpha> (P\<^sup>t \<and>\<alpha> ok')))\<^sup>t)]\<alpha>"
+    by (smt AndA_comm BoolType_aux_var_split okay_simps type_dash)
+
   also from assms
-  have "... = [(p2 \<Rightarrow>\<alpha> ok' (\<alpha> q2) \<and>\<alpha> q2) \<Rightarrow>\<alpha> (p1 \<Rightarrow>\<alpha> ok' (\<alpha> q1) \<and>\<alpha> q1)]\<alpha>"
+  have "... = [(P\<^sup>f \<Leftrightarrow>\<alpha> (P\<^sup>f \<or>\<alpha> (P\<^sup>t \<and>\<alpha> FALSE))) \<and>\<alpha> (P\<^sup>t \<Leftrightarrow>\<alpha> (P\<^sup>f \<or>\<alpha> (P\<^sup>t \<and>\<alpha> TRUE)))]\<alpha>"
+    by (simp add:usubst closure typing alphabet)
+
+  also from assms
+  have "... = [P\<^sup>t \<Leftrightarrow>\<alpha> (P\<^sup>f) \<or>\<alpha> (P\<^sup>t)]\<alpha>"
+    by (simp add:alphabet)
+
+  also from assms have "... = [P\<^sup>f \<Rightarrow>\<alpha> (P\<^sup>t)]\<alpha>"
     apply (utp_alpha_tac)
     apply (utp_pred_auto_tac)
-    (* Need more lemmas to get further ... *)
-    oops
+  done
 
-subsection {* Healthiness Laws properties *}
+  ultimately show ?thesis
+    by simp
+qed
 
-lemma H1_idempotent: "p \<in> WF_RELATION \<Longrightarrow> H1 (H1 p) = H1 p"
-  apply (simp add:H1_def WF_RELATION_def)
-  apply (utp_alpha_tac)
-  apply (utp_pred_tac)
+lemma [simp]: "taut [p]\<alpha> \<longleftrightarrow> taut p"
+  by (utp_alpha_tac, utp_pred_tac)
+
+lemma H2_equivalence':
+  assumes "P \<in> WF_RELATION" "\<alpha> P \<in> DESIGN_ALPHABET"
+          "a \<in> HOM_ALPHABET" "in\<^sub>\<alpha> a = undash `\<^sub>f out\<^sub>\<alpha> (\<alpha> P)"
+  shows "P = (P ;\<alpha> J a) \<longleftrightarrow> taut [P\<^sup>f \<Rightarrow>\<alpha> (P\<^sup>t)]\<alpha>"
+using assms
+  apply (simp add:H2_equivalence[THEN sym])
+  apply (subgoal_tac "\<alpha> P = \<alpha> (P ;\<alpha> J a)")
+  apply (simp add:eq_iff_taut)
+  apply (simp add:alphabet closure alphabet_simps alphabet_dist)
+  apply (metis DESIGN_ALPHABET_finsert(2) HOM_ALPHABET_REL_ALPHABET SemiA_SkipA_right SemiA_alphabet SkipA_alphabet SkipA_closure assms(2))
 done
 
-lemma J_split: 
-  assumes "p \<in> WF_RELATION" 
-  shows "p ;\<alpha> J (\<alpha> p) = p\<^sup>f \<or>\<alpha> (p\<^sup>t \<or>\<alpha> ok' (\<alpha> p))"
+
+lemma [simp]:
+  "`p \<Rightarrow> FALSE` = `\<not> p`" 
+  "`p \<Rightarrow> TRUE` = `true\<^bsub>\<alpha> p\<^esub>`"
+  by (utp_alpha_tac2)+
+
+lemma [simp]:
+  "`p \<oplus> a \<and> q` = `(p \<and> q) \<oplus> a`"
+  "`p \<oplus> a \<or> q` = `(p \<or> q) \<oplus> a`"
+  "`p \<and> q \<oplus> a` = `(p \<and> q) \<oplus> a`"
+  "`p \<or> q \<oplus> a` = `(p \<or> q) \<oplus> a`"
+  by (utp_alpha_tac2)+
+
+lemma [simp]: "a \<in> HOM_ALPHABET \<Longrightarrow> homr a = a"
+  apply (simp add:HOM_ALPHABET_def hom_right_def HOM_ALPHA_unfold alphabet_dist alphabet_simps)
+  apply (metis SkipA_alphabet SkipA_closure WF_RELATION_UNDASHED_DASHED alphabet_simps(14))
+done
+
+lemma [simp]: "a \<in> HOM_ALPHABET \<Longrightarrow> homl a = a"
+  apply (simp add:HOM_ALPHABET_def hom_left_def HOM_ALPHA_unfold alphabet_dist alphabet_simps)
+  apply (metis SkipA_alphabet SkipA_closure WF_RELATION_UNDASHED_DASHED alphabet_simps(14))
+done
+
+lemma J_H2:
+  assumes "a \<in> DESIGN_ALPHABET" "a \<in> HOM_ALPHABET"
+  shows "J a is H2' healthy"
 proof -
-  from assms have "p ;\<alpha> J (\<alpha> p) = p ;\<alpha> (ok (\<alpha> p) \<Rightarrow>\<alpha> ok' (\<alpha> p)) \<and>\<alpha> II\<alpha> (\<alpha> p)"
-    by (simp add: J_def)
 
-  also from assms have "... = p ;\<alpha> (ok (\<alpha> p) \<Rightarrow>\<alpha> ok (\<alpha> p) \<and>\<alpha> ok' (\<alpha> p)) \<and>\<alpha> II\<alpha> (\<alpha> p)"
-    oops
+  from assms have "H2' (J a) = J a ;\<alpha> J a"
+    by (simp add:H2'_def alphabet closure is_healthy_def)
 
-lemma H2_idempotent: "p \<in> WF_RELATION \<Longrightarrow> H2 (H2 p) = H2 p"
-  apply (simp add:H2_def)
-  oops
-
-lemma H3_idempotent: "p \<in> WF_RELATION \<Longrightarrow> H3 (H3 p) = H3 p"
-  apply (simp add:H3_def)
-  oops
-
-lemma H4_idempotent: "p \<in> WF_RELATION \<Longrightarrow> H4 (H4 p) = H4 p"
-  oops
-  
-subsection {* Design Closure Laws *}
-
-(*
-lemma DESIGNS_WF: "DESIGNS \<in> WF_UTP_THEORY"
-proof (simp add:DESIGNS_def WF_UTP_THEORY_def, rule conjI)
-  show wf_alpha:"WF_DESIGN_ALPHABET \<subseteq> WF_ALPHABET"
-    by (force simp add:WF_DESIGN_ALPHABET_def)
-
-  moreover from wf_alpha have "H1 \<in> WF_HEALTH_COND WF_DESIGN_ALPHABET"
-    apply(simp add:WF_HEALTH_COND_def IDEMPOTENT_OVER_def WF_DESIGN_ALPHABET_def)
-    apply(clarify)
-    apply(rule H1_idempotent)
-    apply(simp add: WF_RELATION_def WF_ALPHA_PREDICATE_OVER_def)
+  also from assms have "... = (J a)\<^sup>f \<or>\<alpha> ((J a)\<^sup>t  \<and>\<alpha> ok')"
+    apply (rule_tac J_split)
+    apply (simp_all add:alphabet closure)
+    apply (simp add:HOM_ALPHABET_def, erule conjE)
+    apply (simp add:HOM_ALPHA_unfold)
   done
 
-  moreover from wf_alpha have "H2 \<in> WF_HEALTH_COND WF_DESIGN_ALPHABET"
-    apply(simp add:WF_HEALTH_COND_def IDEMPOTENT_OVER_def WF_DESIGN_ALPHABET_def)
-    apply(clarify)
-    apply(rule H2_idempotent)
-    apply(simp add: WF_RELATION_def WF_ALPHA_PREDICATE_OVER_def)
+  also from assms have "... = `(\<not> ok \<and> II\<^bsub>a -\<^sub>f OK\<^esub>) \<or> (ok' \<and> II\<^bsub>a -\<^sub>f OK\<^esub>)`"
+    (* FIXME: The set simplifiers should be able to cope with this *)
+    apply (subgoal_tac "\<alpha> `((\<not> ok \<and> II\<^bsub>a -\<^sub>f OK\<^esub>) \<or> II\<^bsub>a -\<^sub>f OK\<^esub> \<and> ok')` \<union>\<^sub>f \<lbrace>okay\<rbrace> = 
+                        \<alpha> `((\<not> ok \<and> II\<^bsub>a -\<^sub>f OK\<^esub>) \<or> II\<^bsub>a -\<^sub>f OK\<^esub> \<and> ok')`")
+    apply (simp add:J_def usubst closure alphabet typing)
+    apply (smt AndA_comm)
+    apply (auto simp add:alphabet closure)
   done
 
-  moreover from wf_alpha have "H3 \<in> WF_HEALTH_COND WF_DESIGN_ALPHABET"
-    apply(simp add:WF_HEALTH_COND_def IDEMPOTENT_OVER_def WF_DESIGN_ALPHABET_def)
-    apply(clarify)
-    apply(rule H3_idempotent)
-    apply(simp add: WF_RELATION_def WF_ALPHA_PREDICATE_OVER_def)
+  also from assms have "... = `(\<not> ok \<or> ok') \<and> II\<^bsub>a -\<^sub>f OK\<^esub>`"
+    by (smt AndA_OrA_dist)
+
+  also from assms have "... = `(ok \<Rightarrow> ok') \<and> II\<^bsub>a -\<^sub>f OK\<^esub>`"
+    apply (utp_alpha_tac2)
+    apply (utp_pred_tac)
   done
 
-  moreover from wf_alpha have "H4 \<in> WF_HEALTH_COND WF_DESIGN_ALPHABET"
-    apply(simp add:WF_HEALTH_COND_def IDEMPOTENT_OVER_def WF_DESIGN_ALPHABET_def)
-    apply(clarify)
-    apply(rule H4_idempotent)
-    apply(simp add: WF_RELATION_def WF_ALPHA_PREDICATE_OVER_def)
-  done
-
-
-  ultimately show "{H1, H2, H3, H4} \<in> WF_HEALTH_CONDS WF_DESIGN_ALPHABET"
-    by (simp add:WF_HEALTH_CONDS_def)
+  ultimately show ?thesis
+    by (simp add:is_healthy_def J_def)
 qed
-*)
 
-lemma H1_closure[closure]: 
-"p \<in> WF_ALPHA_PREDICATE \<Longrightarrow> H1 p \<in> WF_ALPHA_PREDICATE"
-  by (simp add:H1_def closure)
+lemma H2_idempotent: 
+  assumes "p \<in> WF_RELATION" "\<alpha> p \<in> DESIGN_ALPHABET"
+  shows "H2' (H2' p) = H2' p"
+proof -
 
+  from assms have "H2' (H2' p) = (p ;\<alpha> J (homr (\<alpha> p))) ;\<alpha> J (homr (\<alpha> p))"
+    apply (simp add:H2'_def alphabet closure)
+    apply (simp add:hom_right_def alphabet alphabet_simps alphabet_dist)
+  done
 
-lemma H2_closure[closure]: 
-"p \<in> WF_ALPHA_PREDICATE \<Longrightarrow> H2 p \<in> WF_ALPHA_PREDICATE"
-  oops
+  also from assms have "... = p ;\<alpha> (J (homr (\<alpha> p)) ;\<alpha> J (homr (\<alpha> p)))"
+    by (metis J_rel_closure REL_ALPHABET_hom_right SemiA_assoc)
 
-subsection {* Alphabet theorems *}
+  also from assms have "... = p ;\<alpha> H2' (J (homr (\<alpha> p)))"
+    by (insert J_H2[of "homr (\<alpha> p)"], simp add:is_healthy_def H2'_def alphabet closure)
 
-subsection {* Design properties *}
- 
+  also from assms have "... = p ;\<alpha> J (homr (\<alpha> p))"
+    by (metis (lifting) DESIGN_ALPHABET_homr HOM_ALPHABET_hom_right J_H2 is_healthy_def)
 
-lemma H1_design: 
-"\<lbrakk> p \<in> WF_ALPHA_PREDICATE; q \<in> WF_ALPHA_PREDICATE \<rbrakk> \<Longrightarrow>
- (p \<turnstile> q) = H1 (p \<turnstile> q)"
-  apply(simp add:DesignD_def H1_def)
-  oops
-*)
+  also from assms have "... = H2' p"
+    by (simp add: H2'_def)
 
+  ultimately show ?thesis
+    by simp
+
+qed
+
+lemma H1_H2_DesignD:
+  assumes cl: "p \<in> WF_RELATION" 
+  and alpha: "\<alpha> p \<in> DESIGN_ALPHABET" 
+  and H1:"p is H1 healthy" 
+  and H2:"p is H2' healthy"
+  shows "p = (\<not>\<alpha> (p\<^sup>f) \<turnstile> (p\<^sup>t))"
+proof -
+
+  have "p = `ok \<Rightarrow> p`"
+    by (metis H1 H1_def is_healthy_def) 
+
+  also have "... = ok \<Rightarrow>\<alpha> (p ;\<alpha> J (homr (\<alpha> p)))"
+    by (metis H2 H2'_def calculation is_healthy_def)
+
+  also have "... = ok \<Rightarrow>\<alpha> ((p\<^sup>f) \<or>\<alpha> (p\<^sup>t \<and>\<alpha> ok'))"
+    apply (insert J_split[of p "homr (\<alpha> p)"])
+    apply (simp add:closure cl alpha)
+    apply (simp add:hom_right_def alphabet_simps alphabet_dist)
+  done
+
+  also have "... = ok \<and>\<alpha> \<not>\<alpha> (p\<^sup>f) \<Rightarrow>\<alpha> ok' \<and>\<alpha> (p\<^sup>t)"
+    by (utp_alpha_tac2, utp_pred_auto_tac)
+
+  ultimately show ?thesis
+    by (simp add:DesignD_def)
+
+qed
+
+   
 end
